DotProduct2: use HReduce

src/examples/GPU.DotProduct2.fst
@@ -11,6 +11,8 @@ module SZ = FStar.SizeT
 module U32 = FStar.UInt32
 module U64 = FStar.UInt64
 
+module HR = GPU.HReduce_U64_Plus
+
 #set-options "--z3rlimit 20"
 
 let size : sz = 1024sz
@@ -22,287 +24,19 @@ let mul (s1 s2: seq u64)
   = Seq.init_ghost (Seq.length s1)
       (fun i -> U64.mul_mod (Seq.index s1 i) (Seq.index s2 i))
 
-[@@ CPrologue "__device__"]
-let spow2 (s : sz{s < 32}) : r:sz{SZ.v r == pow2 (SZ.v s)} =
-  let r = SZ.uint32_to_sizet (U32.shift_left 1ul (sizet_to_u32 s)) in
-  assume (SZ.v r == pow2 (SZ.v s)); // prove this from UInt library
-  r
-
-[@@ CPrologue "__device__"]
-let sdiv_pow2 (i:sz{i < 32}) (tid: sz): bool =
-  SZ.rem tid (spow2 i) = 0sz
-
-[@@ CPrologue "__device__"]
-let smin (a b : sz): sz =
-  let open FStar.SizeT in
-  if a <^ b then a else b
-
-// Pure SUM
-
-let rec sum_seq (s: seq u64) (i j : nat)
-  : Ghost u64 (requires i < j /\ j <= Seq.length s)
-                (ensures fun _ -> True)
-                (decreases j - i)
-=
-  if i = j - 1 then Seq.index s i else U64.add_mod (Seq.index s i) (sum_seq s (i + 1) j)
-
-let add_mod_assoc (a b c: u64): Lemma (U64.add_mod (U64.add_mod a b) c = U64.add_mod a (U64.add_mod b c)) = admit()
-
-let rec sum_seq_lemma (s: seq u64) (i j k:nat):
-  Lemma (requires i < j && j < k && k <= Seq.length s)
-        (ensures sum_seq s i k = U64.add_mod (sum_seq s i j) (sum_seq s j k)) (decreases j - i) =
-    if i = j - 1 then () else (sum_seq_lemma s (i + 1) j k; add_mod_assoc (Seq.index s i) (sum_seq s (i + 1) j) (sum_seq s j k))
-
-// Impure SUM
-
-let gpu_pts_to_slice_sum_inner
-  (#sz:nat)
-  (r: gpu_array u64 sz)
-  (i j:nat)
-  (v: seq u64)
-  (s: seq u64)
-: slprop = gpu_pts_to_array_slice r i j s ** pure (i < j /\ j <= sz /\ Seq.length v = sz /\ Seq.length s = j - i /\ Seq.index s 0 = sum_seq v i j)
-
-let gpu_pts_to_slice_sum
-  (#sz:nat)
-  (r: gpu_array u64 sz)
-  (i j:nat)
-  (v: seq u64)
-: slprop = if_ (i < j && j <= sz) (exists* s. gpu_pts_to_slice_sum_inner #sz r i j v s)
-
-// Barrier
-
-let barrier_matrix (nth: nat) (r : gpu_array u64 nth) (v: seq u64) (it from to: nat): slprop =
-  if_ (from = to + pow2 it)
-      (if_ (not (div_pow2 (it + 1) from) && (div_pow2 it from))
-           (gpu_pts_to_slice_sum r from (min (from + pow2 it) nth) v))
-
-// #push-options "--debug SMTFail --split_queries always"
-// #push-options "--print_implicits"
-
-
-ghost fn unfold_barrier_matrix (nth: nat) (r : gpu_array u64 nth) (v: erased (seq u64))
- (it from to: nat)
-  requires barrier_matrix nth r v it from to
-  ensures  if_ (from = to + pow2 it) (if_ (not (div_pow2 (it + 1) from) && (div_pow2 it from)) (gpu_pts_to_slice_sum r from (min (from + pow2 it) nth) v))
-{
-  unfold (barrier_matrix nth r v it from to)
-}
-
-// let even n : prop = n % 2 == 0
-// let odd  n : prop = ~ (n % 2 == 0)
-
-// let div_helper (n : nat) :
-//   Lemma ((~(even (n+1))) <==>  even n) = ()
-
-val lemma_div_exact: a:int -> p:pos -> Lemma
-  (a % p = 0 <==> a = p * (a / p))
-let lemma_div_exact a p = ()
-
-let div_pow2_lemma_2 (it tid: nat):
-  Lemma (
-    (not (div_pow2 (it + 1) (tid + pow2 it)) && div_pow2 it (tid + pow2 it))
-    <==>
-    div_pow2 (it + 1) tid
-  ) =
-    calc (<==>) {
-      (not (div_pow2 (it + 1) (tid + pow2 it))) && div_pow2 it (tid + pow2 it) <: prop;
-      <==> {}
-      (tid + pow2 it)                       % (2 * pow2 it) <> 0 && (tid + pow2 it) % pow2 it = 0 <: prop;
-      <==> { FStar.Math.Lemmas.lemma_div_mod_plus tid 1 (pow2 it) }
-      (tid + pow2 it)                       % (2 * pow2 it) <> 0 && tid % pow2 it = 0 <: prop;
-      <==> { lemma_div_exact tid (pow2 it) }
-      (pow2 it * (tid / pow2 it) + pow2 it) % (2 * pow2 it) <> 0 && tid % pow2 it = 0 <: prop;
-      <==> { FStar.Math.Lemmas.distributivity_add_right (pow2 it) (tid / pow2 it) 1 }
-      (pow2 it * (tid / pow2 it + 1))       % (2 * pow2 it) <> 0 && tid % pow2 it = 0 <: prop;
-      <==> { FStar.Math.Lemmas.modulo_scale_lemma (tid / pow2 it + 1) (pow2 it) 2 }
-      pow2 it * ((tid / pow2 it + 1) % 2)                   <> 0 && tid % pow2 it = 0 <: prop;
-      <==> {}
-      pow2 it * ((tid / pow2 it) % 2)                        = 0 && tid % pow2 it = 0 <: prop;
-      <==> { FStar.Math.Lemmas.modulo_scale_lemma (tid / pow2 it) (pow2 it) 2 }
-      (pow2 it * (tid / pow2 it)) % (2 * pow2 it)            = 0 && tid % pow2 it = 0 <: prop;
-      <==> { lemma_div_exact tid (pow2 it) }
-      tid % (2 * pow2 it)                                    = 0 && tid % pow2 it = 0 <: prop;
-      <==> { div_pow2_lemma it (it + 1) tid }
-      div_pow2 (it + 1) tid;
-    }
-
-ghost fn fold_barrier_matrix_true
-  (nth : nat)
-  (r: gpu_array u64 nth)
-  (v: seq u64 { Seq.length v == nth })
-  (it: nat)
-  (tid: nat { tid <= nth /\ tid >= pow2 it })
-  (to: nat)
-  requires if_ (to = tid - pow2 it)
-             (if_ (not (div_pow2 (it + 1) tid) && div_pow2 it tid)
-               (gpu_pts_to_slice_sum r tid (min (tid + pow2 it) nth) v))
-  ensures  barrier_matrix nth r v it tid to
-{
-  fold (barrier_matrix nth r v it tid to);
-}
-
-ghost fn fold_barrier_matrix_false
-  (nth : nat)
-  (r: gpu_array u64 nth)
-  (v: seq u64 { Seq.length v == nth })
-  (it: nat)
-  (tid: nat { tid <= nth /\ tid < pow2 it })
-  (to: nat { to <= nth })
-  requires emp
-  ensures  barrier_matrix nth r v it tid to
-{
-  assert (pure (tid < to + pow2 it /\ not (tid = to + pow2 it)));
-  if_intro_false (if_ (not (div_pow2 (it + 1) tid) && (div_pow2 it tid)) (gpu_pts_to_slice_sum r tid (min (tid + pow2 it) nth) v));
-  // (tid = to + pow2 it)
-  fold (barrier_matrix nth r v it tid to);
-}
-
-// #push-options "--print_implicits --print_bound_var_types"
-
-ghost
-fn mk_barrier_pre
-  (nth : sz { 0 < SZ.v nth /\ SZ.v nth <= 1024 })
-  (r : gpu_array u64 nth)
-  (vv: erased (seq u64))
-  (#_: squash (Seq.length vv == nth))
-  (tid : sz{SZ.v tid < nth})
-  (it: sz{it < 31})
-  requires if_ (not (div_pow2 (it + 1) tid) && div_pow2 it tid)
-      (gpu_pts_to_slice_sum #nth r tid (min (tid + pow2 it) nth) vv)
-  ensures bigstar 0 nth (barrier_matrix nth r vv it tid)
-{
-  open FStar.SizeT;
-  if (tid >=^ spow2 it) {
-    bigstar_if_intro 0 nth (tid - pow2 it) (fun _ -> if_ (not (div_pow2 (it + 1) tid) && (div_pow2 it tid)) (gpu_pts_to_slice_sum r tid (min (tid + pow2 it) nth) vv));
-    bigstar_map #_ #_ #0 #nth #(fun (i:nat { 0 <= i /\ i < nth }) -> _ i) (fold_barrier_matrix_true nth r vv it tid);
-  } else {
-    FStar.Math.Lemmas.modulo_lemma tid (spow2 it);
-    FStar.Math.Lemmas.modulo_lemma 0 (spow2 (it +^ 1sz));
-    // assert (pure ((tid <: nat) <> 0 ==> not (div_pow2 it tid)));
-    // assert (pure ((tid <: nat) = 0 ==> (div_pow2 (it + 1) tid)));
-    if_rewrite_bool (op_Negation (div_pow2 (SZ.v it + 1) (SZ.v tid)) && div_pow2 (SZ.v it) (SZ.v tid)) false _;
-    if_elim_false _;
-
-    bigstar_emp_intro 0 nth;
-    bigstar_map #_ #_ #0 #nth #(fun (i:nat { 0 <= i /\ i < nth }) -> emp) (fold_barrier_matrix_false nth r vv it tid);
-  }
-}
-
-#set-options "--print_implicits"
-
-[@@ CPrologue "__device__"]
-fn iteration
-  (nth : sz { 0 < SZ.v nth /\ SZ.v nth <= 1024 })
-  (r : gpu_array u64 nth)
-  (vv: erased (seq u64))
-  (#_: squash (Seq.length vv == nth))
-  (tid : sz{SZ.v tid < nth})
-  (it: sz{it < 31})
-  requires gpu
-    ** mbarrier_tok nth (barrier_matrix nth r vv) it tid
-    ** if_ (div_pow2 it tid) (gpu_pts_to_slice_sum r tid (min (tid + pow2 it) nth) vv)
-  ensures gpu
-    ** mbarrier_tok nth (barrier_matrix nth r vv) (it+1) tid
-    ** if_ (div_pow2 (it+1) tid) (gpu_pts_to_slice_sum r tid (min (tid + pow2 (it + 1)) nth) vv)
-{
-  open FStar.SizeT;
-  assume_ (pure (forall (x:nat). FStar.SizeT.fits x)); // CHEATING overflow
-  assert (pure (Seq.length vv = nth));
-
-  case_split (div_pow2 (it + 1) tid) (if_ (div_pow2 it tid) (gpu_pts_to_slice_sum r tid (min (tid + pow2 it) nth) vv));
-  if_flatten #(div_pow2 (it + 1) tid);
-  if_flatten #(not (div_pow2 (it + 1) tid));
-  
-  div_pow2_lemma it (it + 1) tid;
-  rewrite (if_ (div_pow2 (it + 1) tid && div_pow2 it tid)
-            (gpu_pts_to_slice_sum r tid (min (tid + pow2 it) nth) vv))
-      as (if_ (div_pow2 (it + 1) tid)
-            (gpu_pts_to_slice_sum r tid (min (tid + pow2 it) nth) vv));
-
-  mk_barrier_pre nth r vv tid it;
-  mbarrier_wait #(SZ.v nth) #(barrier_matrix nth r vv) #(SZ.v it) #(SZ.v tid);
-
-  bigstar_map #_ #_ #0 #nth (fun (from: nat { 0 <= from /\ from < nth }) -> unfold_barrier_matrix nth r vv it from tid);
-
-  // combine (div_pow2 (it + 1) tid) (gpu_pts_to_slice_sum r tid (min (tid + pow2 it) nth) vv) _;
-
-  let middle : sz = smin (tid +^ spow2 it) nth;
-  (* We do not use end_ in extracted code, so we can use a nat and erase it
-  so there are no traces in the extracted C. *)
-  let end_   : erased nat = hide (min (tid + 2 * pow2 it) nth);
-
-  if (tid +^ spow2 it <^ nth) {
-    bigstar_if_elim #_ #0
-      #nth (tid + pow2 it)
-      (fun (from: nat) -> if_ (not (div_pow2 (it + 1) from) && (div_pow2 it from)) (gpu_pts_to_slice_sum r from (min (from + pow2 it) nth) vv));
-
-    let b = sdiv_pow2 (it +^ 1sz) tid;
-    
-    assume_ (pure (b <==> (div_pow2 (SZ.v it + 1) (SZ.v tid))));
-    rewrite each (div_pow2 (SZ.v it + 1) (SZ.v tid)) as b;
-
-    div_pow2_lemma_2 it tid;
-    combine
-      b
-      (gpu_pts_to_slice_sum r (tid + pow2 it) (min (tid + pow2 it + pow2 it) nth) vv)
-      _;
-      
-    if b {
-      assert (pure (div_pow2 (SZ.v it + 1) (SZ.v tid)));
-      if_elim_true _;
-
-      unfold (gpu_pts_to_slice_sum r tid middle vv);
-      if_elim_true (exists* s. gpu_pts_to_slice_sum_inner r tid middle vv s);
-      unfold gpu_pts_to_slice_sum_inner;
-      unfold (gpu_pts_to_slice_sum r middle end_ vv);
-      if_elim_true (exists* s. gpu_pts_to_slice_sum_inner r middle end_ vv s);
-      unfold gpu_pts_to_slice_sum_inner;
-
-      let s1 = gpu_array_read #u64 #(SZ.v nth) #(SZ.v tid) #(SZ.v middle) r tid;
-      // assert (pure (s1 == sum_seq vv tid middle));
-      let s2 = gpu_array_read #u64 #(SZ.v nth) #(SZ.v middle) #end_ r middle;
-      // assert (pure (s2 == sum_seq vv middle end_));
-      let s = U64.add_mod s1 s2;
-      sum_seq_lemma vv tid middle end_;
-      // assert (pure ( s == sum_seq vv tid end_ ));
-      gpu_array_write #u64 #(SZ.v nth) #(SZ.v tid) #(SZ.v middle) r tid s;
-
-      gpu_slice_concat #u64 #(SZ.v nth) r tid middle end_;
-      with seq. assert (gpu_pts_to_array_slice r tid end_ seq);
-      // assert (pure (Seq.index seq 0 == s));
-      fold (gpu_pts_to_slice_sum_inner #nth r tid end_ vv seq);
-      if_intro_true (exists* s. gpu_pts_to_slice_sum_inner #nth r tid end_ vv s);
-      fold (gpu_pts_to_slice_sum r tid end_ vv);
-      if_intro_true (gpu_pts_to_slice_sum r tid end_ vv);
-    } else {
-      if_elim_false _;
-      if_intro_false (gpu_pts_to_slice_sum r tid end_ vv);
-    }
-  } else {
-    bigstar_map #_ #_ #0 #nth #(fun (from:nat { 0 <= from /\ from < nth }) -> _ from)
-      (fun (from: nat{0 <= from /\ from < nth}) ->
-        if_rewrite_bool (from = tid + pow2 it) false _);
-    bigstar_map #_ #_ #0 #nth #(fun (from:nat { 0 <= from /\ from < nth }) -> _ from)
-      (fun (from: nat{0 <= from /\ from < nth}) ->
-        if_elim_false (if_ (not (div_pow2 (it + 1) from) && (div_pow2 it from)) (gpu_pts_to_slice_sum r from (min (from + pow2 it) nth) vv)));
-    bigstar_emp_elim #_;
-  }
-}
-
-let kpre (nth: nat) (ga1 ga2 r : gpu_array u64 nth) (#s1 #s2: erased (seq u64))
+let kpre (nth: nat) (ga1 ga2 r : gpu_array u64 nth) (s1 s2: erased (seq u64))
   (#_: squash ( Seq.length s1 == nth /\ Seq.length s2 == nth )) (tid:nat{tid < nth})
   : slprop =
     (gpu_pts_to_array #u64 #nth ga1 #(1.0R /. Real.of_int nth) s1 **
     gpu_pts_to_array #u64 #nth ga2 #(1.0R /. Real.of_int nth) s2) **
     gpu_pts_to_array1 r tid
 
-let kpost (nth: nat) (ga1 ga2 r : gpu_array u64 nth) (#s1 #s2: erased (seq u64))
+let kpost (nth: nat) (ga1 ga2 r : gpu_array u64 nth) (s1 s2: erased (seq u64))
   (#_: squash ( Seq.length s1 == nth /\ Seq.length s2 == nth )) (tid:nat{tid < nth})
   : slprop =
     ((gpu_pts_to_array #u64 #nth ga1 #(1.0R /. Real.of_int nth) s1 **
     gpu_pts_to_array #u64 #nth ga2 #(1.0R /. Real.of_int nth) s2) **
-    if_ (tid = 0) (gpu_pts_to_slice_sum r 0 nth (mul s1 s2)))
+    if_ (tid = 0) (HR.gpu_pts_to_slice_sum r 0 nth (mul s1 s2)))
 
 // #set-options "--ext pulse:env_on_err=1"
 
@@ -314,12 +48,20 @@ fn kernel
   (#s1 #s2: erased (seq u64))
   (#_: squash ( Seq.length s1 == nth /\ Seq.length s2 == nth ))
   (etid : erased tid_t { (gdim_x etid <: nat) == 1ul /\ (bdim_x etid <: nat) == SZ.sizet_to_uint32 nth })
-  requires gpu ** thread_id etid ** mbarrier_tok nth (barrier_matrix nth r (mul s1 s2)) 0 (tidx_x etid) ** kpre  nth ga1 ga2 r #s1 #s2 (thread_index etid)
-  ensures  gpu ** thread_id etid ** (exists* it. mbarrier_tok nth (barrier_matrix nth r (mul s1 s2)) it (tidx_x etid)) ** kpost nth ga1 ga2 r #s1 #s2 (thread_index etid)
+  requires
+    gpu **
+    thread_id etid **
+    mbarrier_tok nth (HR.barrier_matrix nth r (mul s1 s2)) 0 (tidx_x etid) **
+    kpre nth ga1 ga2 r s1 s2 (thread_index etid)
+  ensures
+    gpu **
+    thread_id etid **
+    (exists* it. mbarrier_tok nth (HR.barrier_matrix nth r (mul s1 s2)) it (tidx_x etid)) **
+    kpost nth ga1 ga2 r s1 s2 (thread_index etid)
 {
   let tid = thread_idx_x ();
   let tid : sz = SZ.uint32_to_sizet tid;
-  (**)unfold (kpre nth ga1 ga2 r #s1 #s2 tid);
+  (**)unfold (kpre nth ga1 ga2 r s1 s2 tid);
 
   (**)unfold (gpu_pts_to_array #u64 #(SZ.v nth) ga1 #(1.0R /. Real.of_int nth) s1);
   let v1 = gpu_array_read #u64 #(SZ.v nth) #0 #(SZ.v nth) ga1 tid #s1;
@@ -330,50 +72,24 @@ fn kernel
   (**)fold (gpu_pts_to_array #u64 #nth ga2 #(1.0R /. Real.of_int nth) s2);
   
   let vm = U64.mul_mod v1 v2;
-  let dot_v = hide (mul s1 s2);
+  (**)let dot_v = hide (mul s1 s2);
   
   (**)unfold (gpu_pts_to_array1 r tid);
   gpu_array_write #u64 #(SZ.v nth) #(SZ.v tid) #(hide (SZ.v tid+1)) r tid vm;
   
-  (* Reduction *)
-  let mut n = 0sz;
-
-  (**)with s. assert (gpu_pts_to_array_slice r tid (tid+1) s);
-  (**)fold (gpu_pts_to_slice_sum_inner #nth r tid (tid+1) dot_v s);
-  (**)if_intro_true (exists* s. gpu_pts_to_slice_sum_inner #nth r tid (tid + pow2 0) dot_v s);
-  (**)fold (gpu_pts_to_slice_sum r tid (tid + pow2 0) dot_v);
-  (**)if_intro_true (gpu_pts_to_slice_sum r tid (tid + pow2 0) dot_v);
-
-  open FStar.SizeT;
-  while (let it = !n; (spow2 it <^ nth))
-    invariant c.
-    exists* (it:sz).
-      gpu **
-      pts_to n it **
-      mbarrier_tok nth (barrier_matrix nth r dot_v) it tid **
-      if_ (div_pow2 (SZ.v it) (SZ.v tid)) (gpu_pts_to_slice_sum r tid (min (tid + pow2 it) nth) dot_v) **
-      pure (c == (pow2 it < nth) /\ SZ.v it < 31)
-  {
-    let it = !n <: nat;
-    iteration nth r dot_v tid it;
-    assume_ (pure (SZ.v it < 30)); // FIXME: overflow
-    n := it +^ 1sz;
-  };
+  (* sigh... this is terrible. It's a one element sequence. *)
+  with s'. assert (gpu_pts_to_array_slice r tid (tid+1) s');
+  assert (pure (vm == Seq.index dot_v tid));
+  assert (pure (Seq.index s' 0 == vm));
+  assert (pure (Seq.length s' == 1));
+  GPU.Seq.Common.lem_one_elem s' vm; (* oof *)
+  assert (pure (s' == seq![vm <: u64])); (* the freaking refinement made this very difficult. *)
+  rewrite each s' as seq![vm <: u64];
   
-  (**)let it = !n;
-  (**)FStar.Math.Lemmas.modulo_lemma tid (pow2 it);
-  // assert (pure (pow2 it >= nth /\ tid < nth /\ (div_pow2 it tid) == (tid = 0)));
-
-  // rewrite (if_ (div_pow2 (reveal it) tid) (gpu_pts_to_slice_sum r tid (min (tid + pow2 (reveal it)) nth) dot_v))
-  //     as  (if_ (tid = 0) (gpu_pts_to_slice_sum r tid nth dot_v));
-
-  if (tid = 0sz) {
-    (**)if_elim_true (gpu_pts_to_slice_sum r tid (min (tid + pow2 it) nth) dot_v);
-    (**)if_intro_true (gpu_pts_to_slice_sum r 0 nth dot_v);
-    (**)fold (kpost nth ga1 ga2 r #s1 #s2 tid);
-  } else {
-    (**)fold (kpost nth ga1 ga2 r #s1 #s2 tid);
-  };
+  (* Reduction *)
+  GPU.HReduce_U64_Plus.kernel nth r #dot_v #() etid;
+  
+  fold (kpost nth ga1 ga2 r s1 s2 tid);
 }
 
 let shared_array (#nth : nat { nth <> 0 }) (ga : gpu_array u64 nth) (#v: seq u64 { Seq.length v == nth }) (_: nat): slprop =
@@ -409,7 +125,7 @@ fn main
   (#_: squash (Seq.length v1 = size /\ Seq.length v2 = size))
   requires cpu ** A.pts_to a1 v1 ** A.pts_to a2 v2
   returns  dp: u64
-  ensures  cpu ** A.pts_to a1 v1 ** A.pts_to a2 v2 ** pure (dp == sum_seq (mul v1 v2) 0 size)
+  ensures  cpu ** A.pts_to a1 v1 ** A.pts_to a2 v2 ** pure (dp == HR.sum (mul v1 v2))
 {
   let ar = A.alloc #u64 0UL size;
 
@@ -435,32 +151,32 @@ fn main
                  shared_array #size ga2 #v2 i) **
                  gpu_pts_to_array1 gr i)))
   as
-    (bigstar 0 size (fun i -> kpre size ga1 ga2 gr #v1 #v2 i))
+    (bigstar 0 size (fun i -> kpre size ga1 ga2 gr v1 v2 i))
     by tadmit ();
   (**)bigstar_uneta ();
 
   rewrite
     bigstar 0 size
-      (kpre size ga1 ga2 gr #v1 #v2)
+      (kpre size ga1 ga2 gr v1 v2)
   as
     bigstar 0 (1 * SZ.v size)
-      (kpre size ga1 ga2 gr #v1 #v2);
+      (kpre size ga1 ga2 gr v1 v2);
 
   launch_kernel_n_m_barrier #0 1sz size
-    #(kpre size ga1 ga2 gr #v1 #v2)
-    #(kpost size ga1 ga2 gr #v1 #v2)
-    #(barrier_matrix size gr (mul v1 v2))
+    #(kpre size ga1 ga2 gr v1 v2)
+    #(kpost size ga1 ga2 gr v1 v2)
+    #(HR.barrier_matrix size gr (mul v1 v2))
     (fun etid -> kernel size ga1 ga2 gr #v1 #v2 etid);
 
   (**)bigstar_eta ();
   // TODO:
   (**)drop_
-        (bigstar 0 (1 * SZ.v size) (fun i -> kpost size ga1 ga2 gr #v1 #v2 i));
+        (bigstar 0 (1 * SZ.v size) (fun i -> kpost size ga1 ga2 gr v1 v2 i));
   (**)assume_
         (bigstar 0 size
           (fun i -> ((gpu_pts_to_array #u64 #size ga1 #(1.0R /. Real.of_int size) v1 **
                     gpu_pts_to_array #u64 #size ga2 #(1.0R /. Real.of_int size) v2) **
-                    if_ (i = 0) (gpu_pts_to_slice_sum gr 0 size (mul v1 v2)))
+                    if_ (i = 0) (HR.gpu_pts_to_slice_sum gr 0 size (mul v1 v2)))
         ));
   
   (**)bigstar_unzip 0 size _ _;
@@ -471,11 +187,11 @@ fn main
   (**)bigstar_uneta () #0 #0 #size #(shared_array #size ga2 #v2);
   gather_array ga2;
 
-  bigstar_if_elim #_ #0 #size 0 (fun _ -> gpu_pts_to_slice_sum #size gr 0 size (mul v1 v2));
+  bigstar_if_elim #_ #0 #size 0 (fun _ -> HR.gpu_pts_to_slice_sum #size gr 0 size (mul v1 v2));
 
-  unfold gpu_pts_to_slice_sum;
+  unfold HR.gpu_pts_to_slice_sum;
   if_elim_true _;
-  unfold gpu_pts_to_slice_sum_inner;
+  unfold HR.gpu_pts_to_slice_sum_inner;
   with res. assert (gpu_pts_to_array_slice gr 0 size res);
   fold (gpu_pts_to_array #u64 #size gr #1.0R res);
 
