src/lib/GPU.Seq.Common.fst
@@ -13,3 +13,8 @@ let lem_append_slice (#a:Type) (s : seq a) (i j k : nat)
   : Lemma (requires i <= j /\ j <= k /\ k <= length s)
           (ensures append (slice s i j) (slice s j k) == slice s i k)
   = assert (Seq.equal (append (slice s i j) (slice s j k)) (slice s i k))
+
+let lem_one_elem (#a:Type) (s : seq a) (v : a)
+  : Lemma (requires length s == 1 /\ s @! 0 == v)
+          (ensures s == seq![v])
+  = assert (Seq.equal s seq![v])
